add model for omp team

concurrency/common/HybridMachine.v
@@ -6,7 +6,6 @@ Require Import compcert.common.AST.     (*for typ*)
 Require Import compcert.common.Values. (*for val*)
 Require Import compcert.common.Globalenvs.
 Require Import compcert.lib.Integers.
-
 Require Import VST.msl.Axioms.
 Require Import Coq.ZArith.ZArith.
 (*Require Import VST.concurrency.common.core_semantics.*)
@@ -27,11 +26,15 @@ Require Import VST.concurrency.common.coinductive_safety.*)
 
 (* Require Import VST.veric.res_predicates. *)
 (* Require Import VST.veric.Clight_new. *)
-
 Require Import VST.concurrency.common.HybridMachineSig.
 (* Require Import VST.concurrency.CoreSemantics_sum. *)
-Import Maps.
 
+From stdpp Require Import base fin_maps.
+
+Import -(notations) Maps.
+(* avoid conflicts with stdpp.base *)
+Notation "a !!!! b" := (PMap.get b a) (at level 1).
+Import ListNotations.
 
 Module DryHybridMachine.
   Import Events ThreadPool.
@@ -245,7 +248,7 @@ Module DryHybridMachine.
             (** release the lock *)
             (Hstore: Mem.store Mptr m1 b (Ptrofs.intval ofs) (Vptrofs Ptrofs.one) = Some m')
             (HisLock: lockRes tp (b, Ptrofs.intval ofs) = Some rmap)
-            (Hrmap: forall b ofs, rmap.1 !! b ofs = None /\ rmap.2 !! b ofs = None)
+            (Hrmap: forall b ofs, rmap.1 !!!! b ofs = None /\ rmap.2 !!!! b ofs = None)
             (Hangel1: permMapJoin newThreadPerm.1 virtueLP.1 (getThreadR cnt0).1)
             (Hangel2: permMapJoin newThreadPerm.2 virtueLP.2 (getThreadR cnt0).2)
             (Htp': tp' = updThread cnt0 (Kresume c Vundef)
@@ -342,7 +345,7 @@ Module DryHybridMachine.
             (** If this address is a lock*)
             (His_lock: lockRes tp (b, (Ptrofs.intval ofs)) = Some rmap)
             (** And the lock is taken *)
-            (Hrmap: forall b ofs, rmap.1 !! b ofs = None /\ rmap.2 !! b ofs = None)
+            (Hrmap: forall b ofs, rmap.1 !!!! b ofs = None /\ rmap.2 !!!! b ofs = None)
             (** Install the thread's lock permissions*)
             (Hrestrict_pmap: restrPermMap (Hcompat tid0 cnt0).2 = m1)
             (** To free the lock the thread must have at least Writable on it*)
@@ -639,7 +642,124 @@ Module DryHybridMachine.
     
   End DryHybridMachine.
 
-  
+From stdpp Require Import list.
+  Section OpenMPThreads.
+    
+    (* OpenMP thread info *)
+    Record ot_info := {
+      t_tid : nat; (* thread id *)
+      o_team_id : nat; (* each of new team should get a different number *)
+      (* o_tid : nat; thread id in the current team, NOT tid *)
+      (* o_level : nat; nesting level *)
+      o_done : bool (* if it is spawned by some primary thread, set to true when 
+                     it has reached the last barrier *)
+    }.
+
+    Section OpenMPTeam.
+
+    (* team id -> team_tree *) 
+
+    (**   (0)
+
+           parallel(3)-> 
+
+           [0]
+        /  |  \   
+      [(0), (1), (2)]]
+
+            parallel(2) ->
+
+           [0]
+        /    |    \   
+      [(0), [1], (2)]]
+            / \
+    [(0),[(0),(1)], (2)]]      
+            
+    *)
+
+      (* model of the dynamics of a team. Only the leaf threads are executing, the parents are for bookkeeping. *)
+      Inductive team_tree :=
+      | TeamLeaf : ot_info -> team_tree
+      (* parent thread and the including itself *)
+      | TeamNode : ot_info -> (* parent thread *)
+                   list team_tree -> (* the team that it spawns, 
+                                        first thread is same as parent thread but o_tid=0 *)
+                   team_tree.
+
+      (* the first thread in the program *)
+      Definition ot_init (tid: nat) := Build_ot_info tid 0 false.
+
+      (* a team starts with just the main thread *)
+      Definition team_init (tid: nat) := TeamLeaf (ot_init tid).
+
+      (* ot creates a new team with the other team_mates *)
+      Definition spawn_team' (ot: ot_info) (team_mates: list nat) : team_tree :=
+        TeamNode ot $ (λ tid, TeamLeaf (Build_ot_info tid 0 false)) <$> (cons (ot.(t_tid)) team_mates).
+
+      Definition is_tid (tid: nat) (ot: ot_info) :=
+        ot.(t_tid) = tid.
+      #[global] Instance is_tid_dec (tid: nat) (ot: ot_info) : Decision (is_tid tid ot).
+      Proof. apply Nat.eq_dec. Qed.
+
+      (* the list of all leaf threads *)
+      Fixpoint tree_to_list (tree: team_tree) : (list ot_info) :=
+        match tree with
+        | TeamLeaf ot => nil
+        | TeamNode ot ts => concat (map tree_to_list ts)
+        end.
+
+      Definition has_tid (tid: nat) (tree: team_tree) : Prop :=
+        In tid $ map t_tid $ tree_to_list tree.
+
+      Definition get_ot (tid: nat) (tree: team_tree) : option ot_info :=
+        find (λ ot, decide (ot.(t_tid) = tid)) $ tree_to_list tree.
+
+      Definition tid_unique (tree: team_tree) : Prop :=
+        NoDup $ map t_tid $ tree_to_list tree.
+
+      (* `tree` and `tids` contain the same tid, where `tids` is the  *)
+      Definition matching_tids (tree: team_tree) (tids: list nat) : Prop :=
+        ∀ tid, In tid tids ↔ has_tid tid tree.
+
+      Class team_tree_inv (tree: team_tree) : Prop :=
+        { inv_tid_unique    : tid_unique tree;
+          inv_matching_tids : matching_tids tree (map t_tid $ tree_to_list tree) }.
+
+      (** folloing opeartions assume that tids in the trees are NoDup, and the indexing tid exists as a leaf
+           node in the tree. *)
+      (** spawns a team at every TeamLeaf that contains tid.
+       * should require that tid is unique in tree.
+       *)
+      Fixpoint spawn_team (tid: nat) (team_mates: list nat) (tree: team_tree) : team_tree :=
+        match tree with
+        | TeamLeaf ot => if decide $ is_tid tid ot then spawn_team' ot team_mates else tree
+        | TeamNode p ts => TeamNode p $ map (spawn_team tid team_mates) ts
+        end.
+
+      (* a spawned team is done when all team members are done *)
+      Definition team_done (tid: nat) (tree: team_tree) : Prop :=
+        ∃ p ts,
+          tree = TeamNode p ts ∧ 
+          Forall (λ t, ∃ ot, t=TeamLeaf ot ∧ (* all team members must be leaf *)
+                             decide (ot.(o_done) = true)) ts.
+
+      (** assume tid is the primary thread of some team, turn that TeamNode to TeamLeaf.
+       * Happens when all threads, including primary, are done in this team.
+      *)
+      Fixpoint fire_team (tid: nat) (tree: team_tree) : team_tree :=
+        match tree with
+        | TeamLeaf _ => tree
+        | TeamNode p ts => if decide $ is_tid tid p then TeamLeaf p else TeamNode p $ map (fire_team tid) ts
+        end.
+    End OpenMPTeam.
+
+    Section OpenMPStmt.
+      Inductive MetaStmt :=
+      | MParallel : MetaStmt -> MetaStmt
+      | MStmt : Clight.statement -> MetaStmt
+      (* | MFor *)
+      .
+    End OpenMPStmt.
   
   Section HybDryMachineLemmas.
 
